$\begin{matrix}
    e^{-q(u)} = u                           & 
    {S(x)\over y\bigl(q(u)\bigr)} = 1 - u   \\
    q(u) = -ln(u), \;      
    {\begin{align} 
    0 \lt u & \lt 1, \\ 
    u & \le 1 - S(x) \\ 
    \end{align}}                            & 
    y\bigl(q(u)\bigr) = {S(x)\over 1 - u}   \\
\end{matrix}$

$\begin{matrix}
    e^{-J(q)} = S(1 - e^{-q})               & 
    {S(x)\over y(q)} = 1 - e^{-q}           & 
    \alpha(x) := ln(\frac{-xS'(x)}{S(x)})   \\
    J(q) := -ln(S(1 - e^{-q})),\; q \gt 0   & 
    y(q) := {S(x)\over 1 - e^{-q}},\; 
    {\begin{align} 
    q & \gt 0, \\ 
    q & \ge -ln(1-S(x)) \\ 
    \end{align}}                            \\
\end{matrix}$ 

${\begin{align}
q & \gt 0 \\
 & \ge -ln(1-S(x)) \\ 
\end{align}}$